systems/AggregatorDynamic.v
@@ -68,19 +68,17 @@ exact: m_eq_dec.
 Defined.
 
 Record Data := mkData { 
-  local : m ; 
-  aggregate : m ; 
-  adjacent : NS ; 
-  sent : NM ; 
-  received : NM 
+  local : m ;
+  aggregate : m ;
+  adjacent : NS ;
+  balance : NM
 }.
 
 Definition InitData :=
   {| local := 1 ;
      aggregate := 1 ;
      adjacent := NSet.empty ;
-     sent := NMap.empty m ;
-     received := NMap.empty m |}.
+     balance := NMap.empty m |}.
 
 Definition Handler (S : Type) := GenHandler unit S Output unit.
 
@@ -89,52 +87,46 @@ st <- get ;;
 match i with
 | Aggregate src m_inp =>  
   when (NSet.mem src st.(adjacent))
-  (match NMap.find src st.(received) with
+  (match NMap.find src st.(balance) with
   | None => nop
   | Some m_src => 
     put {| local := st.(local) ;
            aggregate := st.(aggregate) * m_inp ;
            adjacent := st.(adjacent) ;
-           sent := st.(sent) ;
-           received := NMap.add src (m_src * m_inp) st.(received) |}                                                           
+           balance := NMap.add src (m_src * (m_inp)^-1) st.(balance) |}                                                           
   end)
 | Fail src =>
   when (NSet.mem src st.(adjacent))
-  (match NMap.find src st.(sent), NMap.find src st.(received) with
-  | Some m_snt, Some m_rcd =>    
+  (match NMap.find src st.(balance) with
+  | Some m_bal =>
     put {| local := st.(local) ;
-           aggregate := st.(aggregate) * m_snt * (m_rcd)^-1 ;
+           aggregate := st.(aggregate) * m_bal ;
            adjacent := NSet.remove src st.(adjacent) ;
-           sent := NMap.remove src st.(sent) ;
-           received := NMap.remove src st.(received) |}           
-  | _, _ => nop    
+           balance := NMap.remove src st.(balance) |}           
+  | None => nop
   end)
 | New src =>
   when (~~ NSet.mem src st.(adjacent))
   (put {| local := st.(local) ;
          aggregate := st.(aggregate) ;
          adjacent := NSet.add src st.(adjacent) ;
-         sent := NMap.add src 1 st.(sent) ;
-         received := NMap.add src 1 st.(received)      
-      |})
+         balance := NMap.add src 1 st.(balance) |})
 | Local m_inp =>
   put {| local := m_inp ;
          aggregate := st.(aggregate) * m_inp * st.(local)^-1 ;
          adjacent := st.(adjacent) ;
-         sent := st.(sent) ;
-         received := st.(received) |}
+         balance := st.(balance) |}
 | AggregateRequest =>  
   write_output (AggregateResponse st.(aggregate))
 | SendAggregate dst =>
   when (NSet.mem dst st.(adjacent) && sumbool_not _ _ (m_eq_dec st.(aggregate) 1))
-  (match NMap.find dst st.(sent) with
-   | None => nop
+  (match NMap.find dst st.(balance) with
    | Some m_dst =>        
      put {| local := st.(local) ;
             aggregate := 1 ;
             adjacent := st.(adjacent) ;
-            sent := NMap.add dst (m_dst * st.(aggregate)) st.(sent) ;
-            received := st.(received) |}
+            balance := NMap.add dst (m_dst * st.(aggregate)) st.(balance) |}
+   | None => nop
    end)
 end.
 
@@ -154,27 +146,23 @@ Instance Aggregator_SingleNodeParams : SingleNodeParams Aggregator_BaseParams :=
 Lemma IOHandler_cases :
   forall i st u out st' ms,
       IOHandler i st = (u, out, st', ms) ->
-      (exists m_inp m_src src, i = Aggregate src m_inp /\ NSet.In src st.(adjacent) /\ NMap.find src st.(received) = Some m_src /\
+      (exists m_inp m_src src, i = Aggregate src m_inp /\ NSet.In src st.(adjacent) /\ NMap.find src st.(balance) = Some m_src /\
        st'.(local) = st.(local) /\
        st'.(aggregate) = st.(aggregate) * m_inp /\
        st'.(adjacent) = st.(adjacent) /\
-       st'.(sent) = st.(sent) /\     
-       st'.(received) = NMap.add src (m_src * m_inp) st.(received) /\
+       st'.(balance) = NMap.add src (m_src * (m_inp)^-1) st.(balance) /\
        out = []) \/
-      (exists m_inp src, i = Aggregate src m_inp /\ NSet.In src st.(adjacent) /\ NMap.find src st.(received) = None /\ 
+      (exists m_inp src, i = Aggregate src m_inp /\ NSet.In src st.(adjacent) /\ NMap.find src st.(balance) = None /\ 
        st' = st /\ out = []) \/
       (exists m_inp src, i = Aggregate src m_inp /\ ~ NSet.In src st.(adjacent) /\
        st' = st /\ out = []) \/
-      (exists m_snt m_rcd src, i = Fail src /\ NSet.In src st.(adjacent) /\ NMap.find src st.(sent) = Some m_snt /\ NMap.find src st.(received) = Some m_rcd /\
+      (exists m_bal src, i = Fail src /\ NSet.In src st.(adjacent) /\ NMap.find src st.(balance) = Some m_bal /\
        st'.(local) = st.(local) /\ 
-       st'.(aggregate) = st.(aggregate) * m_snt * (m_rcd)^-1 /\
+       st'.(aggregate) = st.(aggregate) * m_bal /\
        st'.(adjacent) = NSet.remove src st.(adjacent) /\
-       st'.(sent) = NMap.remove src st.(sent) /\
-       st'.(received) = NMap.remove src st.(received) /\
+       st'.(balance) = NMap.remove src st.(balance) /\
        out = []) \/
-      (exists src, i = Fail src /\ NSet.In src st.(adjacent) /\ NMap.find src st.(received) = None /\
-       st' = st /\ out = []) \/
-      (exists src, i = Fail src /\ NSet.In src st.(adjacent) /\ NMap.find src st.(sent) = None /\
+      (exists src, i = Fail src /\ NSet.In src st.(adjacent) /\ NMap.find src st.(balance) = None /\
        st' = st /\ out = []) \/
       (exists src, i = Fail src /\ ~ NSet.In src st.(adjacent) /\
        st' = st /\ out = []) \/
@@ -182,8 +170,7 @@ Lemma IOHandler_cases :
        st'.(local) = st.(local) /\ 
        st'.(aggregate) = st.(aggregate) /\
        st'.(adjacent) = NSet.add src st.(adjacent) /\
-       st'.(sent) = NMap.add src 1 st.(sent) /\
-       st'.(received) = NMap.add src 1 st.(received) /\
+       st'.(balance) = NMap.add src 1 st.(balance) /\
        out = []) \/
       (exists src, i = New src /\ NSet.In src st.(adjacent) /\
        st' = st /\ out = []) \/
@@ -191,17 +178,15 @@ Lemma IOHandler_cases :
        st'.(local) = m_inp /\ 
        st'.(aggregate) = st.(aggregate) * m_inp * st.(local)^-1 /\ 
        st'.(adjacent) = st.(adjacent) /\
-       st'.(sent) = st.(sent) /\
-       st'.(received) = st.(received) /\
+       st'.(balance) = st.(balance) /\
        out = []) \/
-      (exists dst m', i = SendAggregate dst /\ NSet.In dst st.(adjacent) /\ st.(aggregate) <> 1 /\ NMap.find dst st.(sent) = Some m' /\
+      (exists dst m_bal, i = SendAggregate dst /\ NSet.In dst st.(adjacent) /\ st.(aggregate) <> 1 /\ NMap.find dst st.(balance) = Some m_bal /\
          st'.(local) = st.(local) /\ 
          st'.(aggregate) = 1 /\
          st'.(adjacent) = st.(adjacent) /\
-         st'.(sent) = NMap.add dst (m' * st.(aggregate)) st.(sent) /\
-         st'.(received) = st.(received) /\
+         st'.(balance) = NMap.add dst (m_bal * st.(aggregate)) st.(balance) /\
          out = []) \/
-      (exists dst, i = SendAggregate dst /\ NSet.In dst st.(adjacent) /\ st.(aggregate) <> 1 /\ NMap.find dst st.(sent) = None /\
+      (exists dst, i = SendAggregate dst /\ NSet.In dst st.(adjacent) /\ st.(aggregate) <> 1 /\ NMap.find dst st.(balance) = None /\
          st' = st /\
          out = []) \/
       (exists dst, i = SendAggregate dst /\ ~ NSet.In dst st.(adjacent) /\ 
@@ -230,28 +215,25 @@ case: i => [src m_inp|src|src|m_inp|dst|]; monad_unfold.
   repeat break_match; repeat tuple_inversion.
   * find_apply_lem_hyp NSetFacts.mem_2.
     right; right; right; left => /=.
-    by exists a; exists a0; exists src.
+    by exists a; exists src.
   * find_apply_lem_hyp NSetFacts.mem_2.
     right; right; right; right; left => /=.
     by exists src.
-  * find_apply_lem_hyp NSetFacts.mem_2.
-    right; right; right; right; right; left => /=.
-    by exists src.
   * have H_ins: ~ NSet.In src st'.(adjacent) by move => H_ins; find_apply_lem_hyp NSetFacts.mem_1; eauto.
-    right; right; right; right; right; right; left => /=.
+    right; right; right; right; right; left => /=.
     by exists src.
 - move => H_eq.
   repeat break_let; break_match; repeat tuple_inversion.
   * have H_ins: ~ NSet.In src st.(adjacent) by move => H_ins; find_apply_lem_hyp NSetFacts.mem_1; rewrite H_ins in Heqb.
-    right; right; right; right; right; right; right; left => /=.
+    right; right; right; right; right; right; left => /=.
     by exists src.
   * move/negP/negP: Heqb => Heqb.
     find_apply_lem_hyp NSetFacts.mem_2.
-    right; right; right; right; right; right; right; right; left => /=.
+    right; right; right; right; right; right; right; left => /=.
     by exists src.
 - move => H_eq.
   repeat tuple_inversion.
-  right; right; right; right; right; right; right; right; right; left => /=.
+  right; right; right; right; right; right; right; right; left => /=.
   by exists m_inp.
 - move => H_eq.
   repeat break_let; break_if; first (repeat break_let; break_match).
@@ -260,29 +242,29 @@ case: i => [src m_inp|src|src|m_inp|dst|]; monad_unfold.
     rewrite /sumbool_not in H_neq.
     break_match => //.
     find_apply_lem_hyp NSetFacts.mem_2.
-    right; right; right; right; right; right; right; right; right; right; left => /=.
+    right; right; right; right; right; right; right; right; right; left => /=.
     by exists dst; exists a.
   * move/andP: Heqb => /= [H_mem H_neq].
     repeat tuple_inversion.
     rewrite /sumbool_not in H_neq.
     break_match => //.
     find_apply_lem_hyp NSetFacts.mem_2.
-    right; right; right; right; right; right; right; right; right; right; right; left => /=.
+    right; right; right; right; right; right; right; right; right; right; left => /=.
     by exists dst.
   * move/nandP: Heqb => /= Heqb.
     repeat tuple_inversion.
     break_or_hyp.
       move/negP: H => H.
       have H_ins: ~ NSet.In dst st'.(adjacent) by move => H_ins; find_apply_lem_hyp NSetFacts.mem_1.
-      right; right; right; right; right; right; right; right; right; right; right; right; left => /=.
+      right; right; right; right; right; right; right; right; right; right; right; left => /=.
       by exists dst.
     unfold sumbool_not in *.
     break_match => //.
-    right; right; right; right; right; right; right; right; right; right; right; right; right; left => /=.
+    right; right; right; right; right; right; right; right; right; right; right; right; left => /=.
     by exists dst.
 - move => H_eq.
   tuple_inversion.
-  by right; right; right; right; right; right; right; right; right; right; right; right; right; right.
+  by right; right; right; right; right; right; right; right; right; right; right; right; right.
 Qed.
 
 Ltac io_handler_cases := 
@@ -291,14 +273,8 @@ Ltac io_handler_cases :=
   intuition idtac; subst; 
   repeat find_rewrite.
 
-Instance AggregationData_Data : AggregationData Data :=
-  {
-    aggr_local := local ;
-    aggr_aggregate := aggregate ;
-    aggr_adjacent := adjacent ;
-    aggr_sent := sent ;
-    aggr_received := received
-  }.
+Definition conserves_node_mass (d : data) : Prop := 
+d.(local) = d.(aggregate) * sumM d.(adjacent) d.(balance).
 
 Lemma Aggregator_conserves_node_mass : 
  forall st tr, step_s_star init_handler st tr ->
@@ -307,7 +283,10 @@ Proof.
 move => st tr H_st.
 remember init_handler as y in *.
 move: Heqy.
-induction H_st using refl_trans_1n_trace_n1_ind => H_init; first by rewrite H_init /conserves_node_mass /InitData; gsimpl.
+induction H_st using refl_trans_1n_trace_n1_ind => H_init.
+  rewrite H_init /conserves_node_mass /InitData /init_handler /=.
+  rewrite sumM_empty; first by gsimpl.
+  exact NSetFacts.empty_1.
 concludes.
 match goal with
 | [ H : step_s _ _ _ |- _ ] => invc H
@@ -320,18 +299,19 @@ io_handler_cases; unfold conserves_node_mass in *; simpl in * => //.
   rewrite sumM_add_map //; gsimpl.
   set m1 := aggregate _.
   set m2 := sumM _ _.
-  set m3 := sumM _ _.
-  suff H_suff: m1 * x * m2 * x^-1 * m3^-1 = m1 * m2 * m3^-1 * (x * x^-1) by rewrite H_suff; gsimpl.
+  set rhs := _ * _ * _.
+  suff H_suff: rhs = m1 * m2 * (x * x^-1) by rewrite H_suff; gsimpl.
+  rewrite /rhs.
   by aac_reflexivity.
 - repeat find_rewrite.  
-  rewrite (sumM_remove_remove H H1) (sumM_remove_remove H H2); gsimpl.
+  rewrite (sumM_remove_remove H H1); gsimpl.
   set m1 := aggregate _.
   set m2 := sumM _ _.
-  set m3 := sumM _ _.
-  suff H_suff: m1 * x * x0^-1 * m2 * x^-1 * x0 * m3^-1 = m1 * m2 * m3^-1 * (x * x^-1) * (x0 * x0^-1) by rewrite H_suff; gsimpl.
+  set rhs := _ * _ * _.
+  suff H_suff: rhs = m1 * m2 * (x * x^-1) by rewrite H_suff; gsimpl.
+  rewrite /rhs.
   by aac_reflexivity.
 - repeat find_rewrite.
-  rewrite sumM_add_add //.
   rewrite sumM_add_add //.
   by gsimpl.
 - repeat find_rewrite.
@@ -339,13 +319,14 @@ io_handler_cases; unfold conserves_node_mass in *; simpl in * => //.
   set m0 := local _.
   set m1 := aggregate _.
   set m2 := sumM _ _.
-  set m3 := sumM _ _.
-  suff H_suff: m1 * m0 * m2 * m3^-1 * m1^-1 * m3 * m2^-1 = m0 * (m1 * m1^-1) * (m2 * m2^-1) * (m3 * m3^-1) by rewrite H_suff; gsimpl.
+  set rhs := _ * _.
+  suff H_suff: rhs = m0 * (m1 * m1^-1) * (m2 * m2^-1) by rewrite H_suff; gsimpl.
+  rewrite /rhs.
   by aac_reflexivity.
 - repeat find_rewrite.
   rewrite sumM_add_map //.
   gsimpl.
   by aac_reflexivity.
-Qed. 
+Qed.
 
 End SingleAggregator.
